dropping a ref.

theories/typing/unsafe/refcell/ref_code.v
@@ -10,6 +10,40 @@ Set Default Proof Using "Type".
 Section ref_functions.
   Context `{typeG Σ, refcellG Σ}.
 
+  Lemma refcell_inv_reading_inv tid l γ α ty q ν :
+    refcell_inv tid l γ α ty -∗
+    own γ (◯ reading_st q ν) -∗
+    ∃ q' q'' n, l ↦ #(Zpos n) ∗
+            own γ (● Some (Cinr (to_agree ν, q', n)) ⋅ ◯ reading_st q ν) ∗
+            ⌜(q' + q'' = 1)%Qp ∧ (q ≤ q')%Qc⌝ ∗ q''.[ν] ∗
+            ty.(ty_shr) (α ∪ ν) tid (shift_loc l 1) ∗
+            ((1).[ν] ={⊤,⊤ ∖ ↑lftN}▷=∗ &{α} shift_loc l 1 ↦∗: ty_own ty tid).
+  Proof.
+    iIntros "INV H◯".
+    iDestruct "INV" as (st) "(H↦lrc & H● & INV)".
+    iAssert (∃ q' n, st ≡ Some (Cinr (to_agree ν, q', n)) ∗ ⌜q ≤ q'⌝%Qc)%I with
+       "[#]" as (q' n) "[Hst %]".
+    { iDestruct (own_valid_2 with "H● H◯") as %[[[=]|
+         (? & st' & [=<-] & -> & [Heq|Hle])]%option_included Hv]%auth_valid_discrete_2.
+      - iExists q, xH.  iSplit; iPureIntro. by constructor. done.
+      - iClear "∗#".
+        revert Hle Hv=>/csum_included [ -> // | [[?[?[//]]] | [?[st''[Heq[-> Hle]]]]]].
+        revert Heq. intros [= <-]. destruct st'' as [[ag q'] n].
+        revert Hle=>/Some_included_2 /Some_pair_included
+           [/Some_pair_included_total_1 [/agree_included Heq Hqq'] _] [[Hag _] _].
+        iExists q', n. iSplit.
+        + iPureIntro. do 4 constructor; last done.
+          apply agree_op_inv. by rewrite comm -Heq.
+        + revert Hqq'. by intros [<-%leibniz_equiv|?%frac_included_weak]%Some_included. }
+    iDestruct "Hst" as %[st' [-> Hst']]%equiv_Some_inv_r'.
+    destruct st' as [|[[]]|]; try by inversion Hst'. apply (inj Cinr), (inj2 pair) in Hst'.
+    destruct Hst' as [[Hst' <-%leibniz_equiv]%(inj2 pair) <-%leibniz_equiv].
+    simpl. setoid_rewrite <-Hst'. clear Hst'.
+    iDestruct "INV" as (q'' ν') "(Hag & Hq'q'' & Hν & INV)".
+    iDestruct "Hag" as %<-%(inj to_agree)%leibniz_equiv.
+    iDestruct "Hq'q''" as %Hq'q''. iExists _, _, _. rewrite own_op. iFrame. auto.
+  Qed.
+
   (* Cloning a ref. We need to increment the counter. *)
   Definition ref_clone : val :=
     funrec: <> ["x"] :=
@@ -42,34 +76,17 @@ Section ref_functions.
     iMod (na_bor_acc with "LFT H◯inv Hα2 Hna") as "(H◯ & Hna & Hcloseα2)"; [solve_ndisj..|].
     rewrite {1}heap_mapsto_vec_cons heap_mapsto_vec_singleton.
     iMod "H↦" as "[H↦1 H↦2]". wp_read. wp_let.
-    iDestruct "INV" as (st) "(H↦lrc & H● & INV)". wp_read. wp_let. wp_op. wp_write.
-    iAssert (∃ q' n, st ≡ Some (Cinr (to_agree ν, q', n)))%I with "[#]" as (q' n) "Hst".
-    { iDestruct (own_valid_2 with "H● H◯") as %[[[=]|
-         (? & st' & [=<-] & -> & [Heq|Hle])]%option_included Hv]%auth_valid_discrete_2.
-      - iExists q, xH. iPureIntro. constructor. done.
-      - iClear "∗#".
-        revert Hle Hv=>/csum_included [ -> // | [[?[?[//]]] | [?[st''[Heq[-> Hle]]]]]].
-        revert Heq. intros [= <-]. destruct st'' as [[ag q'] n].
-        revert Hle=>/Some_included_2 /Some_pair_included
-               [/Some_pair_included_total_1 [/agree_included Heq _] _] [[Hag _] _].
-        iExists q', n. iPureIntro. repeat constructor. apply Cinlr_equiv.
-        do 2 constructor; last done. apply agree_op_inv. by rewrite comm -Heq. }
-    iDestruct "Hst" as %[st' [-> Hst']]%equiv_Some_inv_r'.
-    destruct st' as [|[[]]|]; try by inversion Hst'. apply (inj Cinr), (inj2 pair) in Hst'.
-    destruct Hst' as [[Hst' <-%leibniz_equiv]%(inj2 pair) <-%leibniz_equiv].
-    simpl. setoid_rewrite <-Hst'. clear Hst'.
-    iDestruct "INV" as (q'' ν') "(Hag & Hq'q'' & [Hν1 Hν2] & INV)".
-    iDestruct "Hag" as %<-%(inj to_agree)%leibniz_equiv.
-    iDestruct "Hq'q''" as %Hq'q''.
+    iDestruct (refcell_inv_reading_inv with "INV H◯")
+      as (q' q'' n) "(H↦lrc & [H● H◯] & Hq'q'' & [Hν1 Hν2] & INV)".
+    wp_read. wp_let. wp_op. wp_write. iDestruct "Hq'q''" as %[Hq'q'' _].
     iMod (own_update with "H●") as "[H● ?]".
     { apply auth_update_alloc,
          (op_local_update_discrete _ _ (reading_st (q''/2)%Qp ν))=>-[[Hagv _]_].
-      split; [split|].
+      split; [split|done].
       - by rewrite /= agree_idemp.
       - change ((q''/2+q')%Qp ≤ 1%Qp)%Qc. rewrite -Hq'q'' comm -{2}(Qp_div_2 q'').
         apply Qcplus_le_mono_l. rewrite -{1}(Qcplus_0_l (q''/2)%Qp).
-        apply Qcplus_le_mono_r, Qp_ge_0.
-      - done. }
+        apply Qcplus_le_mono_r, Qp_ge_0. }
     wp_bind (new [ #2])%E. iApply wp_new; [done..|]. iNext. iIntros (lr ?) "(%&?&Hlr)".
     iAssert (lx' ↦∗{qlx'} [ #lv; #lrc])%I  with "[H↦1 H↦2]" as "H↦".
     { rewrite heap_mapsto_vec_cons heap_mapsto_vec_singleton. iFrame. }
@@ -128,6 +145,67 @@ Section ref_functions.
     { rewrite tctx_interp_cons tctx_interp_singleton tctx_hasty_val tctx_hasty_val' //.
       iFrame. iApply (ty_shr_mono with "LFT [] Hshr"). by iApply lft_incl_glb. }
     intros r. simpl_subst. eapply type_delete; [solve_typing..|].
+    eapply (type_jump [_]); solve_typing.
+  Qed.
+
+  (* Dropping a ref and decrement the count in the corresponding refcell. *)
+  Definition ref_drop : val :=
+    funrec: <> ["x"] :=
+      let: "rc" := !("x" +ₗ #1) in
+      let: "n" := !"rc" in
+      "rc" <- "n" - #1;;
+      Endlft;;
+      delete [ #2; "x"];;
+      let: "r" := new [ #0] in "return" ["r"].
+
+  Lemma ref_drop_type ty :
+    typed_instruction_ty [] [] [] ref_drop
+      (fn (fun α => [☀α])%EL (fun α => [# ref α ty])  (fun α => unit)).
+  Proof.
+    apply type_fn; [apply _..|]. move=>/= α ret arg. inv_vec arg=>x. simpl_subst.
+    iIntros "!# * #HEAP #LFT Hna Hα HL Hk Hx".
+    rewrite {1}/elctx_interp big_sepL_singleton tctx_interp_singleton tctx_hasty_val.
+    destruct x as [[|lx|]|]; try iDestruct "Hx" as "[]". iDestruct "Hx" as "[Hx Hx†]".
+    iDestruct "Hx" as ([|[[|lv|]|][|[[|lrc|]|][]]]) "Hx"; try iDestruct "Hx" as "[_ >[]]".
+    rewrite {1}heap_mapsto_vec_cons heap_mapsto_vec_singleton.
+    iDestruct "Hx" as "[[Hx↦1 Hx↦2] Hx]". wp_op. wp_read. wp_let.
+    iDestruct "Hx" as (ν q γ β ty') "(_ & #Hαβ & #Hinv & Hν & H◯)".
+    iMod (lft_incl_acc with "Hαβ Hα") as (qβ) "[Hβ Hcloseα]". done.
+    iMod (na_bor_acc with "LFT Hinv Hβ Hna") as "(INV & Hna & Hcloseβ)"; [done..|].
+    iDestruct (refcell_inv_reading_inv with "INV [$H◯]")
+      as (q' q'' n) "(H↦lrc & H●◯ & >% & Hν' & Hshr & Hend)".
+    wp_read. wp_let. wp_op. wp_write.
+    iAssert (|={⊤,⊤ ∖ ↑lftN}▷=> refcell_inv tid lrc γ β ty')%I
+      with "[H↦lrc H●◯ Hν Hν' Hshr Hend]" as "INV".
+    { iDestruct (own_valid with "H●◯")
+        as %[[Heq%(inj Cinr)|Hincl%csum_included]%Some_included Hv]%auth_valid_discrete_2.
+      - destruct Heq as [[_ ?%leibniz_equiv]?%leibniz_equiv]. simpl in *. subst.
+        iExists None. iFrame. iMod (own_update with "H●◯") as "$".
+        { apply auth_update_dealloc. rewrite -(right_id None op (Some _)).
+          apply op_local_update_cancellable_empty, _. }
+        iApply "Hend". replace 1%Qp with (q'+q'')%Qp by naive_solver. iFrame.
+      - destruct Hincl as [[=]|[(?&?&[=]&?)|(?&?&[=<-]&[=<-]&[[[ag q0]n']EQ])]].
+        rewrite EQ. destruct EQ as [[EQag ?%leibniz_equiv]?%leibniz_equiv].
+           simpl in *. subst.
+        iAssert (lrc ↦ #(Z.pos n'))%I with "[H↦lrc]" as "H↦lrc".
+        { destruct n'; [|done..]. by rewrite /= Pos.pred_double_succ. }
+        iExists (Some (Cinr (ag, q0, n'))). iFrame. iMod (own_update with "H●◯") as "$".
+        { apply auth_update_dealloc. rewrite -Cinr_op Some_op.
+          apply (op_local_update_cancellable_empty (reading_st q ν)), _. }
+        iExists (q+q'')%Qp, ν. iFrame. iApply step_fupd_intro; first done. iIntros "!>".
+        iSplit; iPureIntro.
+        + apply agree_op_inv. by rewrite comm -EQag.
+        + rewrite assoc (comm _ q0 q). by intuition. }
+    wp_bind Endlft. iApply (wp_fupd_step with "INV"); [done..|]. wp_seq.
+    iIntros "INV !>". wp_seq. iMod ("Hcloseβ" with "[$INV] Hna") as "[Hβ Hna]".
+    iMod ("Hcloseα" with "Hβ") as "Hα".
+    iAssert (elctx_interp [☀ α] qE) with "[Hα]" as "HE".
+    { by rewrite /elctx_interp big_sepL_singleton. }
+    iApply (type_delete _ _ [ #lx ◁ box (uninit 2)]%TC with "HEAP LFT Hna HE HL Hk");
+      [solve_typing..| |]; first last.
+    { rewrite tctx_interp_singleton tctx_hasty_val' //. iFrame. iExists [ #lv;#lrc].
+      rewrite heap_mapsto_vec_cons heap_mapsto_vec_singleton uninit_own. iFrame. auto. }
+    eapply type_new; [solve_typing..|]=>r. simpl_subst.
     eapply (type_jump [_]); solve_typing.
   Qed.
 End ref_functions.
